Changed definition of bir_get_current_statement, some progress in bir_program_valid_stateScript.sml

src/theory/bir-support/bir_program_valid_stateScript.sml
@@ -1,3 +1,7 @@
+(*
+  The notions of valid states and programs, and their uses
+*)
+
 open HolKernel Parse boolLib bossLib;
 open bir_auxiliaryTheory bir_auxiliaryLib;
 open bir_envTheory bir_valuesTheory
@@ -22,11 +26,11 @@ val bir_is_valid_program_def = Define `bir_is_valid_program p <=>
 (* This allows some nice rewrites *)
 Theorem bir_is_valid_labels_blocks_EQ_EL:
   !p n1 n2. (bir_is_valid_labels (BirProgram p) /\ n1 < LENGTH p /\ n2 < LENGTH p /\
-                ((EL n1 p).bb_label = (EL n2 p).bb_label)) ==> (n1 = n2)
+                (bir_label_of_block (EL n1 p) = bir_label_of_block (EL n2 p))) ==> (n1 = n2)
 Proof
   SIMP_TAC list_ss [bir_is_valid_labels_def, bir_labels_of_program_def] >>
   REPEAT STRIP_TAC >>
-  MP_TAC (Q.ISPEC `MAP (\bl. bl.bb_label) (p:('a bir_generic_block_t) list)` listTheory.EL_ALL_DISTINCT_EL_EQ) >>
+  MP_TAC (Q.ISPEC `MAP (\bl. bir_label_of_block bl) (p:(('a, 'b) bir_generic_block_t) list)` listTheory.EL_ALL_DISTINCT_EL_EQ) >>
   ASM_SIMP_TAC list_ss [GSYM LEFT_EXISTS_IMP_THM] >>
   Q.EXISTS_TAC `n1` >> Q.EXISTS_TAC `n2` >>
   ASM_SIMP_TAC list_ss [listTheory.EL_MAP]
@@ -34,17 +38,17 @@ QED
 
 val bir_is_valid_labels_blocks_EQ = store_thm ("bir_is_valid_labels_blocks_EQ",
   ``!p bl1 bl2. (bir_is_valid_labels (BirProgram p) /\ MEM bl1 p /\ MEM bl2 p /\
-                (bl1.bb_label = bl2.bb_label)) ==> (bl1 = bl2)``,
+                (bir_label_of_block bl1 = bir_label_of_block bl2)) ==> (bl1 = bl2)``,
 
 METIS_TAC [listTheory.MEM_EL, bir_is_valid_labels_blocks_EQ_EL]);
 
 
 val bir_get_program_block_info_by_label_valid_THM = store_thm ("bir_get_program_block_info_by_label_valid_THM",
-  ``(!p l. ((bir_get_program_block_info_by_label (BirProgram p) l = NONE) <=> (!bl. MEM bl p ==> (bl.bb_label <> l)))) /\
+  ``(!p l. ((bir_get_program_block_info_by_label (BirProgram p) l = NONE) <=> (!bl. MEM bl p ==> (bir_label_of_block bl <> l)))) /\
 
     (!p l i bl. bir_is_valid_labels (BirProgram p) ==>
           ((bir_get_program_block_info_by_label (BirProgram p) l = SOME (i, bl)) <=>
-           ((i:num) < LENGTH p) /\ (EL i p = bl) /\ (bl.bb_label = l)))``,
+           ((i:num) < LENGTH p) /\ (EL i p = bl) /\ (bir_label_of_block bl = l)))``,
 
 SIMP_TAC (list_ss++boolSimps.EQUIV_EXTRACT_ss) [bir_get_program_block_info_by_label_def,
   INDEX_FIND_EQ_NONE, listTheory.EVERY_MEM, INDEX_FIND_EQ_SOME_0] >>
@@ -60,15 +64,54 @@ FULL_SIMP_TAC arith_ss []);
    Later this is then used to define valid states
    ------------------------------------------------------------------------- *)
 
-val bir_is_valid_pc_def = Define `bir_is_valid_pc p pc =
-   (?i bl. (bir_get_program_block_info_by_label p (pc.bpc_label) = SOME (i, bl)) /\
-           (pc.bpc_index <= LENGTH bl.bb_statements))`;
+Definition bir_is_valid_index_of_block_def:
+  bir_is_valid_index_of_block bl i =
+    case bl of
+    | BBlock_Stmts stmts_bl => (i <= LENGTH stmts_bl.bb_statements)
+    | BBlock_Ext ext_bl => T
+End
+
+Theorem bir_is_valid_index_of_block_0:
+  !bl. bir_is_valid_index_of_block bl 0
+Proof
+  Cases_on `bl` >>
+  fs[bir_is_valid_index_of_block_def]
+QED
+
+(* TODO: Move? *)
+Definition bir_current_block_is_extern_def:
+  bir_current_block_is_extern p pc =
+    ?i bl. bir_get_program_block_info_by_label p pc.bpc_label = SOME (i,bl) /\
+           bir_block_is_extern bl
+End
+Theorem bir_current_block_is_extern_BSExt:
+  !p pc. bir_current_block_is_extern p pc <=>
+         ?rel. bir_get_current_statement p pc = SOME (BSExt rel)
+Proof
+rpt gen_tac >> eq_tac >> (
+  strip_tac
+) >- (
+fs[bir_current_block_is_extern_def, bir_get_current_statement_def] >>
+Cases_on `bl` >> fs[bir_block_is_extern_def]
+) >>
+fs[bir_current_block_is_extern_def, bir_get_current_statement_def] >>
+Cases_on `bir_get_program_block_info_by_label p pc.bpc_label` >> fs[] >>
+Cases_on `x` >> fs[] >>
+Cases_on `r` >> fs[bir_block_is_extern_def] >>
+Cases_on `pc.bpc_index < LENGTH b.bb_statements` >> fs[]
+QED
+
+Definition bir_is_valid_pc_def:
+  bir_is_valid_pc p pc =
+    ?i bl. bir_get_program_block_info_by_label p pc.bpc_label = SOME (i, bl) /\
+           bir_is_valid_index_of_block bl pc.bpc_index
+End
 
 val bir_is_valid_pc_of_valid_blocks = store_thm ("bir_is_valid_pc_of_valid_blocks",
   ``!p pc. bir_is_valid_labels (BirProgram p) ==>
-           (bir_is_valid_pc (BirProgram p) pc <=> (?bl. MEM bl p /\ (pc.bpc_label = bl.bb_label) /\
-             (pc.bpc_index <= LENGTH bl.bb_statements)))``,
-SIMP_TAC std_ss [bir_is_valid_pc_def, bir_get_program_block_info_by_label_valid_THM,
+           (bir_is_valid_pc (BirProgram p) pc <=> (?bl. MEM bl p /\ (pc.bpc_label = bir_label_of_block bl) /\
+             (bir_is_valid_index_of_block bl pc.bpc_index)))``,
+SIMP_TAC std_ss [bir_is_valid_pc_def, bir_is_valid_index_of_block_def, bir_get_program_block_info_by_label_valid_THM,
   listTheory.MEM_EL, GSYM LEFT_EXISTS_AND_THM] >>
 METIS_TAC[]);
 
@@ -84,9 +127,15 @@ val bir_get_current_statement_IS_SOME = store_thm ("bir_get_current_statement_IS
 
 REPEAT GEN_TAC >>
 Cases_on `bir_get_program_block_info_by_label p pc.bpc_label` >> (
-  ASM_SIMP_TAC std_ss [bir_get_current_statement_def, bir_is_valid_pc_def]
+  ASM_SIMP_TAC std_ss [bir_get_current_statement_def, bir_is_valid_pc_def,
+                       bir_is_valid_index_of_block_def]
 ) >>
-SIMP_TAC (arith_ss++QI_ss++pairSimps.gen_beta_ss++boolSimps.LIFT_COND_ss) []);
+SIMP_TAC (arith_ss++QI_ss++pairSimps.gen_beta_ss) [] >>
+Cases_on `SND x` >> (
+  fs[] >>
+  SIMP_TAC (arith_ss++boolSimps.LIFT_COND_ss) []
+)
+);
 
 
 
@@ -95,40 +144,88 @@ SIMP_TAC (arith_ss++QI_ss++pairSimps.gen_beta_ss++boolSimps.LIFT_COND_ss) []);
    to a basic statement
    ------------------------------------------------------------------------- *)
 
-val bir_get_current_statement_SOME_B = store_thm ("bir_get_current_statement_SOME_B",
-  ``!p pc stmt. (bir_get_current_statement p pc = SOME (BStmtB stmt)) <=>
-                (?i bl. (bir_get_program_block_info_by_label p pc.bpc_label = SOME (i, bl)) /\
-                   (pc.bpc_index < LENGTH bl.bb_statements) /\
-                   (stmt = EL pc.bpc_index bl.bb_statements))``,
-
+Theorem bir_get_current_statement_SOME_B:
+  !p pc stmt. bir_get_current_statement p pc = SOME (BSGen (BStmtB stmt)) <=>
+                ?i bl_stmts. bir_get_program_block_info_by_label p pc.bpc_label = SOME (i, BBlock_Stmts bl_stmts) /\
+                  pc.bpc_index < LENGTH bl_stmts.bb_statements /\
+                  stmt = EL pc.bpc_index bl_stmts.bb_statements
+Proof
 REPEAT GEN_TAC >>
 Cases_on `bir_get_program_block_info_by_label p pc.bpc_label` >> (
   ASM_SIMP_TAC std_ss [bir_get_current_statement_def]
 ) >>
-SIMP_TAC (arith_ss++QI_ss++pairSimps.gen_beta_ss++boolSimps.LIFT_COND_ss++holBACore_ss) [] >>
-METIS_TAC[]);
+SIMP_TAC (arith_ss++QI_ss++pairSimps.gen_beta_ss) [] >>
+Cases_on `SND x` >> (
+  fs[]
+) >>
+Cases_on `pc.bpc_index < LENGTH b.bb_statements` >> (
+  fs[]
+) >- (
+  eq_tac >> (
+    rpt strip_tac
+  ) >- (
+    ASSUME_TAC (ISPEC ``b:('a, 'b) bir_generic_stmt_block_t`` bir_generic_stmt_block_t_literal_nchotomy) >>
+    gs[]
+  ) >>
+  gs[]
+) >>
+rpt strip_tac >>
+fs[]
+QED
 
 
-val bir_get_current_statement_SOME_E = store_thm ("bir_get_current_statement_SOME_E",
-  ``!p pc stmt. (bir_get_current_statement p pc = SOME (BStmtE stmt)) <=>
-                (?i bl. (bir_get_program_block_info_by_label p pc.bpc_label = SOME (i, bl)) /\
-                   (pc.bpc_index = LENGTH bl.bb_statements) /\
-                   (stmt = bl.bb_last_statement))``,
-
+Theorem bir_get_current_statement_SOME_E:
+  !p pc stmt. bir_get_current_statement p pc = SOME (BSGen (BStmtE stmt)) <=>
+              ?i bl_stmts. bir_get_program_block_info_by_label p pc.bpc_label = SOME (i, BBlock_Stmts bl_stmts) /\
+                pc.bpc_index = LENGTH bl_stmts.bb_statements /\
+                stmt = bl_stmts.bb_last_statement
+Proof
 REPEAT GEN_TAC >>
 Cases_on `bir_get_program_block_info_by_label p pc.bpc_label` >> (
   ASM_SIMP_TAC std_ss [bir_get_current_statement_def]
 ) >>
-SIMP_TAC (arith_ss++QI_ss++pairSimps.gen_beta_ss++boolSimps.LIFT_COND_ss++holBACore_ss++boolSimps.EQUIV_EXTRACT_ss) []);
+SIMP_TAC (arith_ss++QI_ss++pairSimps.gen_beta_ss) [] >>
+Cases_on `SND x` >> (
+  fs[]
+) >>
+Cases_on `pc.bpc_index < LENGTH b.bb_statements` >> (
+  fs[]
+) >- (
+  rpt strip_tac >>
+  gs[]
+) >>
+eq_tac >> (
+  rpt strip_tac
+) >- (
+  ASSUME_TAC (ISPEC ``b:('a, 'b) bir_generic_stmt_block_t`` bir_generic_stmt_block_t_literal_nchotomy) >>
+  gs[]
+) >> (
+  gs[]
+)
+QED
 
 
-val bir_pc_next_valid = store_thm ("bir_pc_next_valid",
-``!p pc. (bir_is_valid_pc p (bir_pc_next pc)) <=>
-         (?stmt. bir_get_current_statement p pc = SOME (BStmtB stmt))``,
-
-REPEAT STRIP_TAC >>
-SIMP_TAC (std_ss++holBACore_ss) [bir_is_valid_pc_def, bir_pc_next_def,
-  bir_get_current_statement_SOME_B, GSYM arithmeticTheory.LESS_EQ]);
+(* Only holds if current block is not an extern block *)
+Theorem bir_pc_next_valid:
+  !p pc. ~bir_current_block_is_extern p pc ==>
+         (bir_is_valid_pc p (bir_pc_next pc) <=>
+          ?stmt. bir_get_current_statement p pc = SOME (BSGen (BStmtB stmt)))
+Proof
+rpt strip_tac >>
+FULL_SIMP_TAC std_ss [bir_is_valid_pc_def, bir_pc_next_def,
+  bir_get_current_statement_SOME_B, bir_current_block_is_extern_def] >>
+eq_tac >> (
+  rpt strip_tac
+) >- (
+  Cases_on `bl` >- (
+    qexistsl_tac [`i`, `b`] >>
+    gs[bir_is_valid_index_of_block_def]
+  ) >>
+  fs[bir_block_is_extern_def]
+) >>
+qexistsl_tac [`i`, `BBlock_Stmts bl_stmts`] >>
+gs[bir_is_valid_index_of_block_def]
+QED
 
 
 
@@ -142,7 +239,7 @@ val bir_is_valid_pc_block_pc = store_thm ("bir_is_valid_pc_block_pc",
         MEM l (bir_labels_of_program p)``,
 
 SIMP_TAC (std_ss++holBACore_ss) [bir_is_valid_pc_def,
-  bir_get_program_block_info_by_label_MEM, bir_block_pc_def]);
+  bir_get_program_block_info_by_label_MEM, bir_block_pc_def, bir_is_valid_index_of_block_0]);
 
 
 val bir_pc_first_valid = store_thm ("bir_pc_first_valid",
@@ -184,41 +281,62 @@ val bir_state_init_valid = store_thm ("bir_state_init_valid",
 SIMP_TAC (std_ss++holBACore_ss++holBACore_ss) [bir_is_valid_state_def, bir_state_init_def,
   bir_pc_first_valid, bir_env_oldTheory.bir_is_well_typed_env_THM]);
 
+(* TODO: (Re)Move? *)
+Theorem bir_get_current_statement_NONE_BBlock_Ext:
+  !p pc b. bir_get_current_statement p pc = NONE ==>
+  ~(bir_get_current_block p pc = SOME (BBlock_Ext b))
+Proof
+gs[bir_get_current_statement_def, bir_get_current_block_def] >>
+Cases_on `bir_get_program_block_info_by_label p pc.bpc_label` >> (
+  fs[]
+) >>
+rpt strip_tac >>
+Cases_on `x` >> (
+  fs[]
+)
+QED
+
 
 val bir_exec_step_invalid_pc_THM = store_thm ("bir_exec_step_invalid_pc_THM",
- ``!ext_map p st ext_st. ~(bir_is_valid_pc p st.bst_pc) ==>
-          (bir_exec_step ext_map p (st, ext_st) = (if (bir_state_is_terminated st) then st else bir_state_set_failed st, ext_st))``,
-
-METIS_TAC[bir_exec_step_def, bir_get_current_statement_IS_SOME, optionTheory.option_CLAUSES]);
+ ``!p st ext_st.
+   ~bir_is_valid_pc p st.bst_pc ==>
+    (bir_exec_step p (st, ext_st) = (if (bir_state_is_terminated st) then st else bir_state_set_failed st, ext_st))``,
+metis_tac[bir_exec_step_def, bir_get_current_statement_IS_SOME, optionTheory.option_CLAUSES]
+);
 
 
 (* valid states allow some nice rewrite for bir_exec_step *)
-val bir_exec_step_valid_THM = store_thm ("bir_exec_step_valid_THM",
- ``!ext_map p st ext_st. bir_is_valid_pc p st.bst_pc ==>
-          (if bir_state_is_terminated st then
-             (bir_exec_step ext_map p (st, ext_st) = (st, ext_st))
-           else
-             (?stmt. (bir_get_current_statement p st.bst_pc = SOME stmt) /\
-                     (bir_exec_step ext_map p (st, ext_st) = (bir_exec_stmt ext_map p stmt (st,ext_st)))))``,
-
-REPEAT STRIP_TAC >>
-FULL_SIMP_TAC std_ss [bir_exec_step_def] >>
+(* Only holds if current block is not an extern block *)
+Theorem bir_exec_step_valid_THM:
+  !p st ext_st.
+     ~bir_current_block_is_extern p st.bst_pc ==>
+     bir_is_valid_pc p st.bst_pc ==>
+     if bir_state_is_terminated st then
+       bir_exec_step p (st, ext_st) = (st, ext_st)
+     else
+       ?stmt. bir_get_current_statement p st.bst_pc = SOME (BSGen stmt) /\
+              bir_exec_step p (st, ext_st) = bir_exec_stmt p stmt (st,ext_st)
+Proof
+rpt strip_tac >>
+FULL_SIMP_TAC std_ss [bir_exec_step_def, bir_current_block_is_extern_BSExt] >>
 Cases_on `bir_state_is_terminated st` >> ASM_SIMP_TAC (std_ss++boolSimps.CONJ_ss) [] >>
-`IS_SOME (bir_get_current_statement p st.bst_pc)` suffices_by METIS_TAC[optionTheory.IS_SOME_EXISTS] >>
-FULL_SIMP_TAC std_ss [bir_get_current_statement_IS_SOME,
-  bir_is_valid_state_def]);
+fs[GSYM bir_get_current_statement_IS_SOME, optionTheory.IS_SOME_EXISTS] >>
+Cases_on `x` >> fs[]
+QED
 
 
 val bir_exec_step_state_valid_THM = store_thm ("bir_exec_step_state_valid_THM",
- ``!ext_map p st ext_st. bir_is_valid_pc p st.bst_pc ==>
-          (if bir_state_is_terminated st then
-             (bir_exec_step ext_map p (st, ext_st) = (st, ext_st))
-           else
-             (?stmt. (bir_get_current_statement p st.bst_pc = SOME stmt) /\
-                     (bir_exec_step ext_map p (st, ext_st) = (bir_exec_stmt ext_map p stmt (st, ext_st)))))``,
+ ``!p st ext_st.
+     ~bir_current_block_is_extern p st.bst_pc ==>
+     bir_is_valid_pc p st.bst_pc ==>
+     (if bir_state_is_terminated st then
+        (bir_exec_step p (st, ext_st) = (st, ext_st))
+      else
+        (?stmt. (bir_get_current_statement p st.bst_pc = SOME (BSGen stmt)) /\
+                (bir_exec_step p (st, ext_st) = (bir_exec_stmt p stmt (st, ext_st)))))``,
 
 REPEAT STRIP_TAC >>
-MP_TAC (Q.SPECL [`ext_map`, `p`, `st`, `ext_st`] bir_exec_step_valid_THM) >>
+MP_TAC (Q.SPECL [`p`, `st`, `ext_st`] bir_exec_step_valid_THM) >>
 ASM_SIMP_TAC std_ss [bir_exec_step_def, bir_exec_stmt_def]);
 
 
@@ -227,32 +345,33 @@ ASM_SIMP_TAC std_ss [bir_exec_step_def, bir_exec_stmt_def]);
    ------------------------------------------------------------------------- *)
 
 val bir_exec_stmtB_well_typed_env_assign = prove (
-  ``!st ext_map v ex ext_st. bir_is_well_typed_env st.bst_environ ==>
-              bir_is_well_typed_env (bir_exec_stmt_assign ext_map v ex (st,ext_st)).bst_environ``,
+  ``!st v ex ext_st. bir_is_well_typed_env st.bst_environ ==>
+              bir_is_well_typed_env (bir_exec_stmt_assign v ex (st,ext_st)).bst_environ``,
 METIS_TAC[bir_env_oldTheory.bir_is_well_typed_env_THM]);
 
 
 val bir_exec_stmtB_well_typed_env_assert = prove (
-  ``!st ext_map ex ext_st. bir_is_well_typed_env st.bst_environ ==>
-            bir_is_well_typed_env (bir_exec_stmt_assert ext_map ex (st,ext_st)).bst_environ``,
+  ``!st ex ext_st. bir_is_well_typed_env st.bst_environ ==>
+            bir_is_well_typed_env (bir_exec_stmt_assert ex (st,ext_st)).bst_environ``,
 METIS_TAC[bir_env_oldTheory.bir_is_well_typed_env_THM]);
 
 
 val bir_exec_stmtB_well_typed_env_assume = prove (
-  ``!st ext_map ex ext_st. bir_is_well_typed_env st.bst_environ ==>
-            bir_is_well_typed_env (bir_exec_stmt_assume ext_map ex (st,ext_st)).bst_environ``,
+  ``!st ex ext_st. bir_is_well_typed_env st.bst_environ ==>
+            bir_is_well_typed_env (bir_exec_stmt_assume ex (st,ext_st)).bst_environ``,
 METIS_TAC[bir_env_oldTheory.bir_is_well_typed_env_THM]);
 
-
+(*
 val bir_exec_stmtB_well_typed_env_extput = prove (
   ``!st ext_map en ex ext_st.
       bir_is_well_typed_env st.bst_environ ==>
       bir_is_well_typed_env (FST (bir_exec_stmt_ext_put ext_map en ex (st,ext_st))).bst_environ``,
 METIS_TAC[bir_env_oldTheory.bir_is_well_typed_env_THM]);
+*)
 
 val bir_exec_stmtB_well_typed_env = store_thm ("bir_exec_stmtB_well_typed_env",
-``!ext_map st stmt ext_st. bir_is_well_typed_env st.bst_environ ==>
-            bir_is_well_typed_env (FST (bir_exec_stmtB ext_map stmt (st,ext_st))).bst_environ``,
+``!st stmt ext_st. bir_is_well_typed_env st.bst_environ ==>
+            bir_is_well_typed_env (FST (bir_exec_stmtB stmt (st,ext_st))).bst_environ``,
 
 REPEAT STRIP_TAC >>
 Cases_on `stmt` >> (
@@ -265,21 +384,20 @@ Cases_on `stmt` >> (
 
 
 val bir_exec_stmtB_pc_unchanged = store_thm ("bir_exec_stmtB_pc_unchanged",
-``!ext_map st ext_st stmt. (FST (bir_exec_stmtB ext_map stmt (st, ext_st))).bst_pc = st.bst_pc``,
+``!st ext_st stmt. (FST (bir_exec_stmtB stmt (st, ext_st))).bst_pc = st.bst_pc``,
 
 REPEAT STRIP_TAC >>
 Cases_on `stmt` >> (
   ASM_SIMP_TAC std_ss [bir_exec_stmtB_def, LET_DEF,
     bir_exec_stmt_assume_def,
-    bir_exec_stmt_assign_def, bir_exec_stmt_assert_def,
-    bir_exec_stmt_ext_put_def] >>
+    bir_exec_stmt_assign_def, bir_exec_stmt_assert_def] >>
   REPEAT CASE_TAC >>
   FULL_SIMP_TAC (std_ss++holBACore_ss) [bir_state_set_typeerror_def]
 ));
 
 val bir_exec_stmtB_valid_state_invar = store_thm ("bir_exec_stmtB_valid_state_invar",
-``!ext_map p st ext_st stmt. bir_is_valid_state p st ==>
-              bir_is_valid_state p (FST (bir_exec_stmtB ext_map stmt (st, ext_st)))``,
+``!p st ext_st stmt. bir_is_valid_state p st ==>
+              bir_is_valid_state p (FST (bir_exec_stmtB stmt (st, ext_st)))``,
 
 SIMP_TAC std_ss [bir_is_valid_state_def,
   bir_exec_stmtB_pc_unchanged, bir_exec_stmtB_well_typed_env]);
@@ -298,8 +416,8 @@ COND_CASES_TAC >| [
 
 
 val bir_exec_stmt_jmp_valid_pc = store_thm ("bir_exec_stmt_jmp_valid_pc",
-  ``!ext_map p st ext_st l. bir_is_valid_pc p st.bst_pc ==>
-             bir_is_valid_pc p (bir_exec_stmt_jmp ext_map p l (st, ext_st)).bst_pc``,
+  ``!p st ext_st l. bir_is_valid_pc p st.bst_pc ==>
+             bir_is_valid_pc p (bir_exec_stmt_jmp p l (st, ext_st)).bst_pc``,
 SIMP_TAC std_ss [bir_exec_stmt_jmp_def] >>
 REPEAT STRIP_TAC >> CASE_TAC >> (
   ASM_SIMP_TAC (std_ss++bir_TYPES_ss) [
@@ -309,19 +427,19 @@ REPEAT STRIP_TAC >> CASE_TAC >> (
 
 
 val bir_exec_stmtE_valid_pc_jmp = prove (
-  ``!ext_map p st ext_st l. bir_is_valid_pc p st.bst_pc ==>
-             bir_is_valid_pc p (bir_exec_stmtE ext_map p (BStmt_Jmp l) (st, ext_st)).bst_pc``,
+  ``!p st ext_st l. bir_is_valid_pc p st.bst_pc ==>
+             bir_is_valid_pc p (bir_exec_stmtE p (BStmt_Jmp l) (st, ext_st)).bst_pc``,
 SIMP_TAC std_ss [bir_exec_stmtE_def, bir_exec_stmt_jmp_valid_pc]);
 
 
 val bir_exec_stmtE_valid_pc_cjmp = prove (
-  ``!ext_map p st ext_st ex l1 l2.
+  ``!p st ext_st ex l1 l2.
        bir_is_valid_pc p st.bst_pc ==>
-       bir_is_valid_pc p (bir_exec_stmtE ext_map p (BStmt_CJmp ex l1 l2) (st, ext_st)).bst_pc``,
+       bir_is_valid_pc p (bir_exec_stmtE p (BStmt_CJmp ex l1 l2) (st, ext_st)).bst_pc``,
 SIMP_TAC std_ss [bir_exec_stmtE_def, bir_exec_stmt_cjmp_def] >>
 REPEAT STRIP_TAC >>
-Cases_on `option_CASE (bir_eval_exp ext_map ex st.bst_environ ext_st) NONE bir_dest_bool_val` >- (
-  Cases_on `bir_eval_exp ext_map ex st.bst_environ ext_st` >> (
+Cases_on `option_CASE (bir_eval_exp ex st.bst_environ ext_st) NONE bir_dest_bool_val` >- (
+  Cases_on `bir_eval_exp ex st.bst_environ ext_st` >> (
     ASM_SIMP_TAC (std_ss++bir_TYPES_ss) [bir_state_set_typeerror_def, LET_DEF]
   )
 ) >>
@@ -332,20 +450,20 @@ Cases_on `c` >> (
 
 
 val bir_exec_stmtE_valid_pc_halt = prove (
-  ``!ext_map p st ex ext_st.
+  ``!p st ex ext_st.
       bir_is_valid_pc p st.bst_pc ==>
-      bir_is_valid_pc p (bir_exec_stmtE ext_map p (BStmt_Halt ex) (st, ext_st)).bst_pc``,
+      bir_is_valid_pc p (bir_exec_stmtE p (BStmt_Halt ex) (st, ext_st)).bst_pc``,
   SIMP_TAC (std_ss++holBACore_ss) [bir_exec_stmtE_def, bir_exec_stmt_halt_def] >>
   REPEAT STRIP_TAC >>
-  Cases_on `bir_eval_exp ext_map ex st.bst_environ ext_st` >> (
+  Cases_on `bir_eval_exp ex st.bst_environ ext_st` >> (
     ASM_SIMP_TAC (std_ss++bir_TYPES_ss) [bir_state_set_typeerror_def, LET_DEF]
   )
 );
 
 
 val bir_exec_stmtE_valid_pc = store_thm ("bir_exec_stmtE_valid_pc",
-``!ext_map p st ext_st stmt. bir_is_valid_pc p st.bst_pc ==>
-              bir_is_valid_pc p (bir_exec_stmtE ext_map p stmt (st, ext_st)).bst_pc``,
+``!p st ext_st stmt. bir_is_valid_pc p st.bst_pc ==>
+              bir_is_valid_pc p (bir_exec_stmtE p stmt (st, ext_st)).bst_pc``,
 
 REPEAT STRIP_TAC >>
 Cases_on `stmt` >> (
@@ -357,7 +475,7 @@ Cases_on `stmt` >> (
 
 
 val bir_exec_stmtE_env_unchanged = store_thm ("bir_exec_stmtE_env_unchanged",
-``!ext_map p st ext_st stmt. (bir_exec_stmtE ext_map p stmt (st, ext_st)).bst_environ = st.bst_environ``,
+``!p st ext_st stmt. (bir_exec_stmtE p stmt (st, ext_st)).bst_environ = st.bst_environ``,
 
 REPEAT STRIP_TAC >>
 Cases_on `stmt` >> (
@@ -367,7 +485,7 @@ Cases_on `stmt` >> (
     bir_state_set_typeerror_def] >>
   REPEAT CASE_TAC >>
   SIMP_TAC (std_ss++holBACore_ss) [LET_DEF] >>
-  Cases_on `bir_eval_exp ext_map b st.bst_environ ext_st` >> (
+  Cases_on `bir_eval_exp b st.bst_environ ext_st` >> (
     SIMP_TAC (std_ss++holBACore_ss) [LET_DEF]
   ) >> (
     rename1 `bir_dest_bool_val x''` >> Cases_on `bir_dest_bool_val x''`
@@ -381,16 +499,16 @@ Cases_on `stmt` >> (
 
 
 val bir_exec_stmtE_valid_state_invar = store_thm ("bir_exec_stmtE_valid_state_invar",
-``!ext_map p st ext_st stmt. bir_is_valid_state p st ==>
-              bir_is_valid_state p (bir_exec_stmtE ext_map p stmt (st, ext_st))``,
+``!p st ext_st stmt. bir_is_valid_state p st ==>
+              bir_is_valid_state p (bir_exec_stmtE p stmt (st, ext_st))``,
 
 SIMP_TAC std_ss [bir_is_valid_state_def,
   bir_exec_stmtE_env_unchanged, bir_exec_stmtE_valid_pc]);
 
 
 val bir_exec_stmtE_block_pc = store_thm ("bir_exec_stmtE_block_pc",
-``!ext_map p st ext_st stmt. ~(bir_state_is_terminated (bir_exec_stmtE ext_map p stmt (st, ext_st))) ==>
-              ((bir_exec_stmtE ext_map p stmt (st, ext_st)).bst_pc.bpc_index = 0)``,
+``!p st ext_st stmt. ~(bir_state_is_terminated (bir_exec_stmtE p stmt (st, ext_st))) ==>
+              ((bir_exec_stmtE p stmt (st, ext_st)).bst_pc.bpc_index = 0)``,
 
 REPEAT GEN_TAC >>
 Cases_on `stmt` >> (
@@ -400,7 +518,7 @@ Cases_on `stmt` >> (
     bir_state_set_typeerror_def] >>
   REPEAT CASE_TAC >>
   SIMP_TAC (std_ss++holBACore_ss) [bir_block_pc_def, LET_DEF] >>
-  Cases_on `bir_eval_exp ext_map b st.bst_environ ext_st` >> (
+  Cases_on `bir_eval_exp b st.bst_environ ext_st` >> (
     SIMP_TAC (std_ss++holBACore_ss) [bir_block_pc_def, LET_DEF]
   ) >> (
     rename1 `bir_dest_bool_val x''` >> Cases_on `bir_dest_bool_val x''`
@@ -414,7 +532,7 @@ Cases_on `stmt` >> (
 
 
 val bir_exec_step_valid_pc = store_thm ("bir_exec_step_valid_pc",
-``!ext_map p st ext_st. bir_is_valid_pc p (FST (bir_exec_step ext_map p (st, ext_st))).bst_pc <=>
+``!p st ext_st. bir_is_valid_pc p (FST (bir_exec_step p (st, ext_st))).bst_pc <=>
          bir_is_valid_pc p st.bst_pc``,
 
 REPEAT STRIP_TAC >>
@@ -427,17 +545,17 @@ EQ_TAC >> REPEAT STRIP_TAC >- (
   REV_FULL_SIMP_TAC (std_ss++bir_TYPES_ss) [bir_state_set_failed_def]
 ) >>
 IMP_RES_TAC bir_exec_step_state_valid_THM >>
-QSPECL_X_ASSUM ``!ext_st ext_map. _`` [`ext_st`, `ext_map`] >>
+QSPECL_X_ASSUM ``!ext_st. _`` [`ext_st`] >>
 REV_FULL_SIMP_TAC std_ss [] >>
 Cases_on `stmt` >> (
   ASM_SIMP_TAC std_ss [bir_exec_stmt_def, bir_exec_stmtE_valid_pc, LET_DEF]
 ) >>
-rename1 `bir_exec_stmtB ext_map stmt (st, ext_st)` >>
-Q.ABBREV_TAC `st'_tup = bir_exec_stmtB ext_map stmt (st, ext_st)` >>
+rename1 `bir_exec_stmtB stmt (st, ext_st)` >>
+Q.ABBREV_TAC `st'_tup = bir_exec_stmtB stmt (st, ext_st)` >>
 PairCases_on `st'_tup` >>
-rename1 `(st', ext_st') = bir_exec_stmtB ext_map stmt (st,ext_st)` >>
+rename1 `(st', ext_st') = bir_exec_stmtB stmt (st,ext_st)` >>
 subgoal `st'.bst_pc = st.bst_pc` >- (
-  subgoal `(FST (bir_exec_stmtB ext_map stmt (st,ext_st))).bst_pc = st.bst_pc` >- (
+  subgoal `(FST (bir_exec_stmtB stmt (st,ext_st))).bst_pc = st.bst_pc` >- (
     fs[bir_exec_stmtB_pc_unchanged]
   ) >>
   gvs[pairTheory.FST]
